add_mul_pos uses int31 only
git-svn-id: svn+ssh://scm.gforge.inria.fr/svn/coq/trunk@9845 85f007b7-540e-0410-9357-904b9bb8a0f7

theories/Ints/num/GenBase.v
@@ -25,10 +25,14 @@ Section GenBase.
  Variable w_WW  : w -> w -> zn2z w.
  Variable w_0W  : w -> zn2z w.
  Variable w_digits : positive.
+ Variable w_zdigits: w.
+ Variable w_add: w -> w -> zn2z w.
  Variable w_to_Z   : w -> Z.
  Variable w_compare : w -> w -> comparison. 
  
  Definition ww_digits := xO w_digits.
+
+ Definition ww_zdigits := w_add w_zdigits w_zdigits.
 
  Definition ww_to_Z := zn2z_to_Z (base w_digits) w_to_Z.
 
