theories/Ints/num/GenDivn1.v
@@ -20,11 +20,16 @@ Section GENDIVN1.
 
  Variable w             : Set.
  Variable w_digits      : positive.
+ Variable w_zdigits     : w.
  Variable w_0           : w.
  Variable w_WW          : w -> w -> zn2z w.
- Variable w_head0       : w -> N.
- Variable w_add_mul_div : positive -> w -> w -> w.
+ Variable w_head0       : w -> w.
+ Variable w_add_mul_div : w -> w -> w -> w.
  Variable w_div21       : w -> w -> w -> w * w.
+ Variable w_compare     : w -> w -> comparison.
+ Variable w_sub         : w -> w -> w.
+ 
+
  
  (* ** For proofs ** *)
  Variable w_to_Z        : w -> Z.
@@ -37,22 +42,34 @@ Section GENDIVN1.
  Notation "[[ x ]]" := (zn2z_to_Z wB w_to_Z x)  (at level 0, x at level 99).
  
  Variable spec_to_Z   : forall x, 0 <= [| x |] < wB.
+ Variable spec_w_zdigits: [|w_zdigits|] = Zpos w_digits.
  Variable spec_0   : [|w_0|] = 0.
  Variable spec_WW  : forall h l, [[w_WW h l]] = [|h|] * wB + [|l|].
  Variable spec_head0  : forall x,  0 < [|x|] ->
-	 wB/ 2 <= 2 ^ (Z_of_N (w_head0 x)) * [|x|] < wB.
+	 wB/ 2 <= 2 ^ [|w_head0 x|] * [|x|] < wB.
  Variable spec_add_mul_div : forall x y p,
-        Zpos p < Zpos w_digits ->
+        [|p|] <= Zpos w_digits ->
        [| w_add_mul_div p x y |] =
-         ([|x|] * (Zpower 2 (Zpos p)) +
-          [|y|] / (Zpower 2 ((Zpos w_digits) - (Zpos p)))) mod wB.
+         ([|x|] * (2 ^ [|p|]) +
+          [|y|] / (2 ^ ((Zpos w_digits) - [|p|]))) mod wB.
  Variable spec_div21 : forall a1 a2 b,
      wB/2 <= [|b|] ->
      [|a1|] < [|b|] ->
      let (q,r) := w_div21 a1 a2 b in
      [|a1|] *wB+ [|a2|] = [|q|] * [|b|] + [|r|] /\
      0 <= [|r|] < [|b|].
+ Variable spec_compare :
+     forall x y,
+       match w_compare x y with
+       | Eq => [|x|] = [|y|]
+       | Lt => [|x|] < [|y|]
+       | Gt => [|x|] > [|y|]
+       end.
+ Variable spec_sub: forall x y, 
+   [|w_sub x y|] = ([|x|] - [|y|]) mod wB.
+
  
+
  Section DIVAUX.
   Variable b2p : w.
   Variable b2p_le : wB/2 <= [|b2p|].
@@ -117,13 +134,13 @@ Section GENDIVN1.
    rewrite IHn. destruct (gen_divn1_0 n rh hl);trivial.
   Qed.
  
-  Variable p : positive.
-  Variable p_bounded : Zpos p < Zpos w_digits.
+  Variable p : w.
+  Variable p_bounded : [|p|] <= Zpos w_digits.
 
   Lemma spec_add_mul_divp : forall x y,
     [| w_add_mul_div p x y |] =
-       ([|x|] * (Zpower 2 (Zpos p)) +
-          [|y|] / (Zpower 2 ((Zpos w_digits) - (Zpos p)))) mod wB.
+       ([|x|] * (2 ^ [|p|]) +
+          [|y|] / (2 ^ ((Zpos w_digits) - [|p|]))) mod wB.
   Proof.
    intros;apply spec_add_mul_div;auto.
   Qed.
@@ -142,22 +159,26 @@ Section GENDIVN1.
    | S n => gen_divn1_p_aux n (gen_divn1_p n)   
    end.
 
-  Lemma p_lt_gen_digits : forall n, Zpos p < Zpos (gen_digits w_digits n).
+  Lemma p_lt_gen_digits : forall n, [|p|] <= Zpos (gen_digits w_digits n).
   Proof.
+(*
    induction n;simpl. destruct p_bounded;trivial.
-   assert (0 < Zpos p). unfold Zlt;reflexivity.
-   rewrite Zpos_xO;auto with zarith.
+   case (spec_to_Z p); rewrite Zpos_xO;auto with zarith.
+*)
+   induction n;simpl. trivial.
+   case (spec_to_Z p); rewrite Zpos_xO;auto with zarith.
   Qed.
 
   Lemma spec_gen_divn1_p : forall n r h l,
     [|r|] < [|b2p|] ->
     let (q,r') := gen_divn1_p n r h l in
     [|r|] * gen_wB w_digits n + 
-      ([!n|h!]*2^(Zpos p) + 
-        [!n|l!] / (2^(Zpos(gen_digits w_digits n) - Zpos p)))
+      ([!n|h!]*2^[|p|] + 
+        [!n|l!] / (2^(Zpos(gen_digits w_digits n) - [|p|])))
         mod gen_wB w_digits n = [!n|q!] * [|b2p|] + [|r'|] /\
     0 <= [|r'|] < [|b2p|].
   Proof.
+   case (spec_to_Z p); intros HH0 HH1.
    induction n;intros.
    unfold gen_divn1_p, gen_divn1_p_aux, gen_to_Z, gen_wB, gen_digits.
    rewrite <- spec_add_mul_divp.
@@ -168,26 +189,26 @@ Section GENDIVN1.
    assert (H2 := spec_split n l);destruct (gen_split w_0 n l) as (lh,ll).
    rewrite H2.
    replace ([|r|] * (gen_wB w_digits n * gen_wB w_digits n) +
-    (([!n|hh!] * gen_wB w_digits n + [!n|hl!]) * 2 ^ Zpos p +
+    (([!n|hh!] * gen_wB w_digits n + [!n|hl!]) * 2 ^ [|p|] +
     ([!n|lh!] * gen_wB w_digits n + [!n|ll!]) /
-     2^(Zpos (gen_digits w_digits (S n)) - Zpos p)) mod
+     2^(Zpos (gen_digits w_digits (S n)) - [|p|])) mod
       (gen_wB w_digits n * gen_wB w_digits n)) with
-    (([|r|] * gen_wB w_digits n + ([!n|hh!] * 2^Zpos p + 
-      [!n|hl!] / 2^(Zpos (gen_digits w_digits n) - Zpos p)) mod
+    (([|r|] * gen_wB w_digits n + ([!n|hh!] * 2^[|p|] + 
+      [!n|hl!] / 2^(Zpos (gen_digits w_digits n) - [|p|])) mod
                       gen_wB w_digits n) * gen_wB w_digits n +
-     ([!n|hl!] * 2^Zpos p + 
-      [!n|lh!] / 2^(Zpos (gen_digits w_digits n) - Zpos p)) mod 
+     ([!n|hl!] * 2^[|p|] + 
+      [!n|lh!] / 2^(Zpos (gen_digits w_digits n) - [|p|])) mod 
               gen_wB w_digits n).
    generalize (IHn r hh hl H);destruct (gen_divn1_p n r hh hl) as (qh,rh);
    intros (H3,H4);rewrite H3.
    assert ([|rh|] < [|b2p|]). omega. 
    replace (([!n|qh!] * [|b2p|] + [|rh|]) * gen_wB w_digits n +
-     ([!n|hl!] * 2 ^ Zpos p +
-      [!n|lh!] / 2 ^ (Zpos (gen_digits w_digits n) - Zpos p)) mod
+     ([!n|hl!] * 2 ^ [|p|] +
+      [!n|lh!] / 2 ^ (Zpos (gen_digits w_digits n) - [|p|])) mod
       gen_wB w_digits n)  with  
     ([!n|qh!] * [|b2p|] *gen_wB w_digits n + ([|rh|]*gen_wB w_digits n +
-      ([!n|hl!] * 2 ^ Zpos p +
-       [!n|lh!] / 2 ^ (Zpos (gen_digits w_digits n) - Zpos p)) mod
+      ([!n|hl!] * 2 ^ [|p|] +
+       [!n|lh!] / 2 ^ (Zpos (gen_digits w_digits n) - [|p|])) mod
       gen_wB w_digits n)). 2:ring.
    generalize (IHn rh hl lh H0);destruct (gen_divn1_p n rh hl lh) as (ql,rl);
    intros (H5,H6);rewrite H5.
@@ -205,32 +226,32 @@ Section GENDIVN1.
    rewrite Zdiv_shift_r;auto with zarith. 
    2:change (Zpos (gen_digits w_digits (S n))) 
      with (2*Zpos (gen_digits w_digits n));auto with zarith.
-   replace (2 ^ (Zpos (gen_digits w_digits (S n)) - Zpos p)) with
-    (2^(Zpos (gen_digits w_digits n) - Zpos p)*2^Zpos (gen_digits w_digits n)).
+   replace (2 ^ (Zpos (gen_digits w_digits (S n)) - [|p|])) with
+    (2^(Zpos (gen_digits w_digits n) - [|p|])*2^Zpos (gen_digits w_digits n)).
    rewrite Zdiv_Zmult_compat_r;auto with zarith.
-   rewrite Zmult_plus_distr_l with (p:=  2^Zpos p). 
-   pattern  ([!n|hl!] * 2^Zpos p) at 2;
-   rewrite (shift_unshift_mod (Zpos(gen_digits w_digits n))(Zpos p)([!n|hl!]));
+   rewrite Zmult_plus_distr_l with (p:=  2^[|p|]). 
+   pattern  ([!n|hl!] * 2^[|p|]) at 2;
+   rewrite (shift_unshift_mod (Zpos(gen_digits w_digits n))([|p|])([!n|hl!]));
     auto with zarith.
    rewrite Zplus_assoc. 
    replace 
-    ([!n|hh!] * 2^Zpos (gen_digits w_digits n)* 2^Zpos p +
-      ([!n|hl!] / 2^(Zpos (gen_digits w_digits n)-Zpos p)*
+    ([!n|hh!] * 2^Zpos (gen_digits w_digits n)* 2^[|p|] +
+      ([!n|hl!] / 2^(Zpos (gen_digits w_digits n)-[|p|])*
        2^Zpos(gen_digits w_digits n)))
    with 
-    (([!n|hh!] *2^Zpos p + gen_to_Z w_digits w_to_Z n hl / 
-       2^(Zpos (gen_digits w_digits n)-Zpos p))
+    (([!n|hh!] *2^[|p|] + gen_to_Z w_digits w_to_Z n hl / 
+       2^(Zpos (gen_digits w_digits n)-[|p|]))
       * 2^Zpos(gen_digits w_digits n));try (ring;fail).
    rewrite <- Zplus_assoc.
-   rewrite <- (Zmod_shift_r (Zpos p));auto with zarith.
+   rewrite <- (Zmod_shift_r ([|p|]));auto with zarith.
    replace 
      (2 ^ Zpos (gen_digits w_digits n) * 2 ^ Zpos (gen_digits w_digits n)) with
      (2 ^ (Zpos (gen_digits w_digits n) + Zpos (gen_digits w_digits n))).
    rewrite (Zmod_shift_r (Zpos (gen_digits w_digits n)));auto with zarith.
    replace (2 ^ (Zpos (gen_digits w_digits n) + Zpos (gen_digits w_digits n)))
    with (2^Zpos(gen_digits w_digits n) *2^Zpos(gen_digits w_digits n)). 
-   rewrite (Zmult_comm (([!n|hh!] * 2 ^ Zpos p +
-      [!n|hl!] / 2 ^ (Zpos (gen_digits w_digits n) - Zpos p)))).
+   rewrite (Zmult_comm (([!n|hh!] * 2 ^ [|p|] +
+      [!n|hl!] / 2 ^ (Zpos (gen_digits w_digits n) - [|p|])))).
    rewrite  Zmod_Zmult_compat_l;auto with zarith.
    ring. 
    rewrite Zpower_exp;auto with zarith.
@@ -241,12 +262,11 @@ Section GENDIVN1.
    split;auto with zarith.
    apply Zdiv_lt_upper_bound;auto with zarith.
    rewrite <- Zpower_exp;auto with zarith.
-   replace (Zpos p + (Zpos (gen_digits w_digits n) - Zpos p)) with 
+   replace ([|p|] + (Zpos (gen_digits w_digits n) - [|p|])) with 
      (Zpos(gen_digits w_digits n));auto with zarith.
-   assert (0 < Zpos p). unfold Zlt;reflexivity. auto with zarith.
    rewrite <- Zpower_exp;auto with zarith.
-   replace (Zpos (gen_digits w_digits (S n)) - Zpos p) with 
-       (Zpos (gen_digits w_digits n) - Zpos p + 
+   replace (Zpos (gen_digits w_digits (S n)) - [|p|]) with 
+       (Zpos (gen_digits w_digits n) - [|p|] + 
          Zpos (gen_digits w_digits n));trivial.
    change (Zpos (gen_digits w_digits (S n))) with 
     (2*Zpos (gen_digits w_digits n)). ring.
@@ -275,14 +295,14 @@ Section GENDIVN1.
 
  End DIVAUX.
 
- Fixpoint hight (n:nat) : word w n -> w :=
+ Fixpoint high (n:nat) : word w n -> w :=
   match n return word w n -> w with
   | O => fun a => a 
   | S n => 
     fun (a:zn2z (word w n)) =>
      match a with
      | W0 => w_0
-     | WW h l => hight n h
+     | WW h l => high n h
      end
   end.
 
@@ -295,16 +315,16 @@ Section GENDIVN1.
   exact (refl_equal Lt).
  Qed.
 
- Lemma spec_hight : forall n (x:word w n), 
-   [|hight n x|] = [!n|x!] / 2^(Zpos (gen_digits w_digits n) - Zpos w_digits).
+ Lemma spec_high : forall n (x:word w n), 
+   [|high n x|] = [!n|x!] / 2^(Zpos (gen_digits w_digits n) - Zpos w_digits).
  Proof.
   induction n;intros.
-  unfold hight,gen_digits,gen_to_Z.
+  unfold high,gen_digits,gen_to_Z.
   replace (Zpos w_digits - Zpos w_digits) with 0;try ring.
   simpl. rewrite <- (Zdiv_unique [|x|] 1 [|x|] 0);auto with zarith.
   assert (U2 := spec_gen_digits n). 
   assert (U3 : 0 < Zpos w_digits). exact (refl_equal Lt).
-  destruct x;unfold hight;fold hight.
+  destruct x;unfold high;fold high.
   unfold gen_to_Z,zn2z_to_Z;rewrite spec_0.
   rewrite Zdiv_0;trivial.
   apply Zpower_lt_0;auto with zarith.
@@ -330,16 +350,17 @@ Section GENDIVN1.
  Qed.
  
  Definition gen_divn1 (n:nat) (a:word w n) (b:w) := 
-  match w_head0 b with
-  | N0 => gen_divn1_0 b n w_0 a 
-  | Npos p =>
+  let p := w_head0 b in
+  match w_compare p w_0 with
+  | Gt =>
     let b2p := w_add_mul_div p b w_0 in
-    let ha := hight n a in
-    let k := Pminus w_digits p in
+    let ha := high n a in
+    let k := w_sub w_zdigits p in
     let lsr_n := w_add_mul_div k w_0 in 
     let r0 := w_add_mul_div p w_0 ha in
     let (q,r) := gen_divn1_p b2p p n r0 a (gen_0 w_0 n) in
     (q, lsr_n r)
+  | _ => gen_divn1_0 b n w_0 a 
   end.
 
  Lemma spec_gen_divn1 : forall n a b,
@@ -349,131 +370,150 @@ Section GENDIVN1.
     0 <= [|r|] < [|b|].
   Proof.
    intros n a b H. unfold gen_divn1.
-   assert (H0 := spec_head0 H).
-   destruct (w_head0 b).
-   unfold Z_of_N, Zpower in H0.
-   rewrite Zmult_1_l in H0;destruct H0.
-   rewrite <- spec_0 in H.
-   assert (H2 := spec_gen_divn1_0 H0 n a H).
-   rewrite spec_0 in H2;rewrite Zmult_0_l in H2;rewrite Zplus_0_l in H2.
-   exact H2.
-   unfold Z_of_N in H0.
-   assert (HHHH : 0 < Zpos p). unfold Zlt;reflexivity.
-   assert (Zpos p < Zpos w_digits).
-    destruct (Z_lt_le_dec (Zpos p) (Zpos w_digits));trivial.
-    assert (2 ^ Zpos p < wB).
-     apply Zle_lt_trans with (2 ^ Zpos p * [|b|]);auto with zarith.
-     replace (2 ^ Zpos p) with (2^Zpos p * 1);try (ring;fail).
+   case (spec_head0 H); intros H0 H1.
+   case (spec_to_Z (w_head0 b)); intros HH1 HH2.
+   generalize (spec_compare (w_head0 b) w_0); case w_compare;
+     rewrite spec_0; intros H2; auto with zarith.
+   assert (Hv1: wB/2 <= [|b|]).
+     generalize H0; rewrite H2; rewrite Zpower_exp_0;
+       rewrite Zmult_1_l; auto.
+   assert (Hv2: [|w_0|] < [|b|]).
+     rewrite spec_0; auto.
+   generalize (spec_gen_divn1_0 Hv1 n a Hv2).
+   rewrite spec_0;rewrite Zmult_0_l; rewrite Zplus_0_l; auto.
+   contradict H2; auto with zarith.
+   assert (HHHH : 0 < [|w_head0 b|]); auto with zarith.
+   assert ([|w_head0 b|] < Zpos w_digits).
+    case (Zle_or_lt (Zpos w_digits) [|w_head0 b|]); auto; intros HH.
+    assert (2 ^ [|w_head0 b|] < wB).
+     apply Zle_lt_trans with (2 ^ [|w_head0 b|] * [|b|]);auto with zarith.
+     replace (2 ^ [|w_head0 b|]) with (2^[|w_head0 b|] * 1);try (ring;fail).
      apply Zmult_le_compat;auto with zarith.
-     assert (wB <= 2^Zpos p).
+     assert (wB <= 2^[|w_head0 b|]).
      unfold base;apply Zpower_le_monotone;auto with zarith. omega.
-   assert ([|w_add_mul_div p b w_0|] = 2 ^ Zpos p * [|b|]).
-    assert (H2 := spec_add_mul_div b w_0 H1).
-    rewrite spec_0 in H2;rewrite Zdiv_0 in H2;
-    rewrite Zplus_0_r in H2;rewrite Zmult_comm in H2.
-    rewrite Zmod_def_small in H2;auto with zarith.
-    apply Zpower_lt_0;auto with zarith.
-   destruct H0.
-   assert (H4 := spec_to_Z (hight n a)).
+   assert ([|w_add_mul_div (w_head0 b) b w_0|] = 
+               2 ^ [|w_head0 b|] * [|b|]).
+    rewrite (spec_add_mul_div b w_0); auto with zarith.
+    rewrite spec_0;rewrite Zdiv_0; try omega.
+    rewrite Zplus_0_r; rewrite Zmult_comm.
+    rewrite Zmod_def_small; auto with zarith.
+    apply Zpower_lt_0; try omega.
+   assert (H5 := spec_to_Z (high n a)).
    assert 
-    ([|w_add_mul_div p w_0 (hight n a)|]<[|w_add_mul_div p b w_0|]).
-    rewrite H2.
+    ([|w_add_mul_div (w_head0 b) w_0 (high n a)|]
+          <[|w_add_mul_div (w_head0 b) b w_0|]).
+    rewrite H4.
     rewrite spec_add_mul_div;auto with zarith.
     rewrite spec_0;rewrite Zmult_0_l;rewrite Zplus_0_l.
-    assert (([|hight n a|]/2^(Zpos w_digits - Zpos p)) < wB).
+    assert (([|high n a|]/2^(Zpos w_digits - [|w_head0 b|])) < wB).
      apply Zdiv_lt_upper_bound;auto with zarith. 
      apply Zlt_le_trans with wB;auto with zarith.
      pattern wB at 1;replace wB with (wB*1);try ring.
      apply Zmult_le_compat;auto with zarith.
-     assert (H5 := Zpower_lt_0 2 (Zpos w_digits - Zpos p));
+     assert (H6 := Zpower_lt_0 2 (Zpos w_digits - [|w_head0 b|]));
        auto with zarith.
     rewrite Zmod_def_small;auto with zarith.
     apply Zdiv_lt_upper_bound;auto with zarith.
     apply Zlt_le_trans with wB;auto with zarith.
-    apply Zle_trans with (2 ^ Zpos p * [|b|] * 2).
-    rewrite <- wB_div_2;auto with zarith.
+    apply Zle_trans with (2 ^ [|w_head0 b|] * [|b|] * 2).
+    rewrite <- wB_div_2; try omega.
     apply Zmult_le_compat;auto with zarith.
     pattern 2 at 1;rewrite <- Zpower_exp_1.
     apply Zpower_le_monotone;split;auto with zarith.
-   rewrite <- H2 in H0. 
-   assert (H6:= spec_gen_divn1_p H0 H1 n a (gen_0 w_0 n) H5).
-   destruct (gen_divn1_p (w_add_mul_div p b w_0) p n
-             (w_add_mul_div p w_0 (hight n a)) a
+   rewrite <- H4 in H0. 
+   assert (Hb3: [|w_head0 b|] <= Zpos w_digits); auto with zarith. 
+   assert (H7:= spec_gen_divn1_p H0 Hb3 n a (gen_0 w_0 n) H6).
+   destruct (gen_divn1_p (w_add_mul_div (w_head0 b) b w_0) (w_head0 b) n
+             (w_add_mul_div (w_head0 b) w_0 (high n a)) a
              (gen_0 w_0 n)) as (q,r).
    assert (U:= spec_gen_digits n).
-   rewrite spec_gen_0 in H6;trivial;rewrite Zdiv_0 in H6.
-   rewrite Zplus_0_r in H6.
-   rewrite spec_add_mul_div in H6;auto with zarith.
-   rewrite spec_0 in H6;rewrite Zmult_0_l in H6;rewrite Zplus_0_l in H6.
-   assert (([|hight n a|] / 2 ^ (Zpos w_digits - Zpos p)) mod wB
-     = [!n|a!] / 2^(Zpos (gen_digits w_digits n) - Zpos p)).
+   rewrite spec_gen_0 in H7;trivial;rewrite Zdiv_0 in H7.
+   rewrite Zplus_0_r in H7.
+   rewrite spec_add_mul_div in H7;auto with zarith.
+   rewrite spec_0 in H7;rewrite Zmult_0_l in H7;rewrite Zplus_0_l in H7.
+   assert (([|high n a|] / 2 ^ (Zpos w_digits - [|w_head0 b|])) mod wB
+     = [!n|a!] / 2^(Zpos (gen_digits w_digits n) - [|w_head0 b|])).
    rewrite Zmod_def_small;auto with zarith.
-   rewrite spec_hight. rewrite Zdiv_Zdiv;auto with zarith.
+   rewrite spec_high. rewrite Zdiv_Zdiv;auto with zarith.
    rewrite <- Zpower_exp;auto with zarith.
    replace (Zpos (gen_digits w_digits n) - Zpos w_digits + 
-                       (Zpos w_digits - Zpos p))
-    with (Zpos (gen_digits w_digits n) - Zpos p);trivial;ring.
-   assert (H7 := Zpower_lt_0 2  (Zpos w_digits - Zpos p));auto with zarith.
+                       (Zpos w_digits - [|w_head0 b|]))
+    with (Zpos (gen_digits w_digits n) - [|w_head0 b|]);trivial;ring.
+   assert (H8 := Zpower_lt_0 2  (Zpos w_digits - [|w_head0 b|]));auto with zarith.
    split;auto with zarith.
-   apply Zle_lt_trans with ([|hight n a|]);auto with zarith.
+   apply Zle_lt_trans with ([|high n a|]);auto with zarith.
    apply Zdiv_le_upper_bound;auto with zarith.
-   pattern ([|hight n a|]) at 1;rewrite <- Zmult_1_r.
+   pattern ([|high n a|]) at 1;rewrite <- Zmult_1_r.
    apply Zmult_le_compat;auto with zarith.
-   rewrite H7 in H6;unfold gen_wB,base in H6.
-   rewrite <- shift_unshift_mod in H6;auto with zarith.
-   rewrite H2 in H6.
-   assert ([|w_add_mul_div (w_digits - p) w_0 r|] = [|r|]/2^Zpos p).
+   rewrite H8 in H7;unfold gen_wB,base in H7.
+   rewrite <- shift_unshift_mod in H7;auto with zarith.
+   rewrite H4 in H7.
+   assert ([|w_add_mul_div (w_sub w_zdigits (w_head0 b)) w_0 r|] 
+               = [|r|]/2^[|w_head0 b|]).
    rewrite spec_add_mul_div.
    rewrite spec_0;rewrite Zmult_0_l;rewrite Zplus_0_l.
-   replace (Zpos w_digits - Zpos (w_digits - p)) with (Zpos p).
+   replace (Zpos w_digits - [|w_sub w_zdigits (w_head0 b)|]) 
+      with ([|w_head0 b|]).
    rewrite Zmod_def_small;auto with zarith.
-   assert (H8 := spec_to_Z r).
+   assert (H9 := spec_to_Z r).
    split;auto with zarith.
    apply Zle_lt_trans with ([|r|]);auto with zarith.
    apply Zdiv_le_upper_bound;auto with zarith.
    pattern ([|r|]) at 1;rewrite <- Zmult_1_r.
    apply Zmult_le_compat;auto with zarith.
-   assert (H9 := Zpower_lt_0 2  (Zpos p));auto with zarith.
-   rewrite Zpos_minus;auto with zarith.
-   rewrite Zpos_minus;auto with zarith.
-   destruct H6.
+   assert (H10 := Zpower_lt_0 2  ([|w_head0 b|]));auto with zarith.
+   rewrite spec_sub.
+   rewrite Zmod_def_small; auto with zarith.
+   split; auto with zarith.
+   case (spec_to_Z w_zdigits); auto with zarith.
+   rewrite spec_sub.
+   rewrite Zmod_def_small; auto with zarith.
+   split; auto with zarith.
+   case (spec_to_Z w_zdigits); auto with zarith.
+  case H7; intros H71 H72.
    split.
-   rewrite <- (Z_div_mult [!n|a!] (2^Zpos p));auto with zarith.
-   rewrite H8;rewrite H6.
-   replace ([!n|q!] * (2 ^ Zpos p * [|b|])) with ([!n|q!] *[|b|] * 2^Zpos p);
+   rewrite <- (Z_div_mult [!n|a!] (2^[|w_head0 b|]));auto with zarith.
+   rewrite H71;rewrite H9.
+   replace ([!n|q!] * (2 ^ [|w_head0 b|] * [|b|])) 
+      with ([!n|q!] *[|b|] * 2^[|w_head0 b|]);
      try (ring;fail).
    rewrite Z_div_plus_l;auto with zarith.
-   assert (H10 := spec_to_Z (w_add_mul_div (w_digits - p) w_0 r));split;
+   assert (H10 := spec_to_Z 
+       (w_add_mul_div (w_sub w_zdigits (w_head0 b)) w_0 r));split;
     auto with zarith.
-   rewrite H8.
+   rewrite H9.
    apply Zdiv_lt_upper_bound;auto with zarith.
    rewrite Zmult_comm;auto with zarith.
    exact (spec_gen_to_Z w_digits w_to_Z spec_to_Z n a).
    apply Zpower_lt_0;auto with zarith.
  Qed.
 
+ 
  Definition gen_modn1 (n:nat) (a:word w n) (b:w) := 
-  match w_head0 b with
-  | N0 => gen_modn1_0 b n w_0 a 
-  | Npos p =>
+  let p := w_head0 b in
+  match w_compare p w_0 with
+  | Gt =>
     let b2p := w_add_mul_div p b w_0 in
-    let ha := hight n a in
-    let k := Pminus w_digits p in
+    let ha := high n a in
+    let k := w_sub w_zdigits p in
     let lsr_n := w_add_mul_div k w_0 in 
     let r0 := w_add_mul_div p w_0 ha in
     let r := gen_modn1_p b2p p n r0 a (gen_0 w_0 n) in
     lsr_n r
+  | _ => gen_modn1_0 b n w_0 a 
   end.
 
  Lemma spec_gen_modn1_aux : forall n a b,
     gen_modn1 n a b = snd (gen_divn1 n a b).
  Proof.
   intros n a b;unfold gen_divn1,gen_modn1.
-  destruct (w_head0 b).
+  generalize (spec_compare (w_head0 b) w_0); case w_compare;
+     rewrite spec_0; intros H2; auto with zarith.
+  apply spec_gen_modn1_0.
   apply spec_gen_modn1_0.
   rewrite spec_gen_modn1_p.
-  destruct (gen_divn1_p (w_add_mul_div p b w_0) p n
-            (w_add_mul_div p w_0 (hight n a)) a (gen_0 w_0 n));simpl;trivial.
+  destruct (gen_divn1_p (w_add_mul_div (w_head0 b) b w_0) (w_head0 b) n
+            (w_add_mul_div (w_head0 b) w_0 (high n a)) a (gen_0 w_0 n));simpl;trivial.
  Qed.
 
  Lemma spec_gen_modn1 : forall n a b, 0 < [|b|] ->
