theories/Ints/num/GenLift.v
@@ -12,6 +12,7 @@ Require Import ZArith.
 Require Import ZAux.
 Require Import ZPowerAux.
 Require Import ZDivModAux.
+Require Import Zmod.
 Require Import Basic_type.
 Require Import GenBase.
 
@@ -24,47 +25,54 @@ Section GenLift.
  Variable w_W0 : w ->  zn2z w.
  Variable w_0W : w ->  zn2z w.
  Variable w_compare : w -> w -> comparison.
- Variable w_head0 : w -> N.
- Variable w_add_mul_div : positive -> w -> w -> w.
+ Variable ww_compare : zn2z w -> zn2z w -> comparison.
+ Variable w_head0 : w -> w.
+ Variable w_add: w -> w -> zn2z w.
+ Variable w_add_mul_div : w -> w -> w -> w.
+ Variable ww_sub: zn2z w -> zn2z w -> zn2z w.
  Variable w_digits : positive.
  Variable ww_Digits : positive.
+ Variable w_zdigits : w.
+ Variable ww_zdigits : zn2z w.
+ Variable low: zn2z w -> w.
 
  Definition ww_head0 x :=
   match x with
-  | W0 => Npos ww_Digits
+  | W0 => ww_zdigits
   | WW xh xl =>
     match w_compare w_0 xh with
-    | Eq => Nplus (Npos w_digits) (w_head0 xl)
-    | _ => w_head0 xh
+    | Eq => w_add w_zdigits (w_head0 xl)
+    | _ => w_0W (w_head0 xh)
     end
   end.
 
   (* 0 < p < ww_digits *)
  Definition ww_add_mul_div p x y := 
+  let zdigits := w_0W w_zdigits in
   match x, y with
   | W0, W0 => W0
   | W0, WW yh yl =>
-    match Pcompare p w_digits Eq with
+    match ww_compare p zdigits with
     | Eq => w_0W yh 
-    | Lt => w_0W (w_add_mul_div p w_0 yh)
+    | Lt => w_0W (w_add_mul_div (low p) w_0 yh)
     | Gt =>
-      let n := Pminus p w_digits in
+      let n := low (ww_sub p zdigits) in
       w_WW (w_add_mul_div n w_0 yh) (w_add_mul_div n yh yl)
     end
   | WW xh xl, W0 =>
-    match Pcompare p w_digits Eq with
+    match ww_compare p zdigits with
     | Eq => w_W0 xl 
-    | Lt => w_WW (w_add_mul_div p xh xl) (w_add_mul_div p xl w_0)
+    | Lt => w_WW (w_add_mul_div (low p) xh xl) (w_add_mul_div (low p) xl w_0)
     | Gt =>
-      let n := Pminus p w_digits in
+      let n := low (ww_sub p zdigits) in
       w_W0 (w_add_mul_div n xl w_0) 
     end
   | WW xh xl, WW yh yl =>
-    match Pcompare p w_digits Eq with
+    match ww_compare p zdigits with
     | Eq => w_WW xl yh 
-    | Lt => w_WW (w_add_mul_div p xh xl) (w_add_mul_div p xl yh)
+    | Lt => w_WW (w_add_mul_div (low p) xh xl) (w_add_mul_div (low p) xl yh)
     | Gt =>
-      let n := Pminus p w_digits in
+      let n := low (ww_sub p zdigits) in
       w_WW (w_add_mul_div n xl yh) (w_add_mul_div n yh yl)
     end
   end.
@@ -79,6 +87,7 @@ Section GenLift.
 
   Variable spec_w_0   : [|w_0|] = 0.
   Variable spec_to_Z  : forall x, 0 <= [|x|] < wB.
+  Variable spec_to_w_Z  : forall x, 0 <= [[x]] < wwB.
   Variable spec_w_WW : forall h l, [[w_WW h l]] = [|h|] * wB + [|l|].
   Variable spec_w_W0 : forall h, [[w_W0 h]] = [|h|] * wB.
   Variable spec_w_0W : forall l, [[w_0W l]] = [|l|].
@@ -88,47 +97,60 @@ Section GenLift.
        | Lt => [|x|] < [|y|]
        | Gt => [|x|] > [|y|]
        end.
+  Variable spec_ww_compare : forall x y,
+       match ww_compare x y with
+       | Eq => [[x]] = [[y]]
+       | Lt => [[x]] < [[y]]
+       | Gt => [[x]] > [[y]]
+       end.
   Variable spec_ww_digits : ww_Digits = xO w_digits.
   Variable spec_w_head0  : forall x,  0 < [|x|] ->
-	 wB/ 2 <= 2 ^ (Z_of_N (w_head0 x)) * [|x|] < wB.
+	 wB/ 2 <= 2 ^ ([|w_head0 x|]) * [|x|] < wB.
   Variable spec_w_add_mul_div : forall x y p,
-       Zpos p < Zpos w_digits ->
+       [|p|] <= Zpos w_digits ->
        [| w_add_mul_div p x y |] =
-         ([|x|] * (Zpower 2 (Zpos p)) +
-          [|y|] / (Zpower 2 ((Zpos w_digits) - (Zpos p)))) mod wB.
+         ([|x|] * (2 ^ [|p|]) +
+          [|y|] / (2 ^ ((Zpos w_digits) - [|p|]))) mod wB.
+ Variable spec_w_add: forall x y, 
+   [[w_add x y]] = [|x|] + [|y|].
+ Variable spec_ww_sub: forall x y, 
+   [[ww_sub x y]] = ([[x]] - [[y]]) mod wwB.
+
+ Variable spec_zdigits : [| w_zdigits |] = Zpos w_digits.
+ Variable spec_low: forall x, [| low x|] = [[x]] mod wB.
  
 
   Hint Resolve div_le_0 div_lt w_to_Z_wwB: lift.
   Ltac zarith := auto with zarith lift.
    
   Lemma spec_ww_head0  : forall x,  0 < [[x]] ->
-	 wwB/ 2 <= 2 ^ (Z_of_N (ww_head0 x)) * [[x]] < wwB.
+	 wwB/ 2 <= 2 ^ [[ww_head0 x]] * [[x]] < wwB.
   Proof.
    rewrite wwB_div_2;rewrite Zmult_comm;rewrite wwB_wBwB.
    assert (U:= lt_0_wB w_digits); destruct x as [ |xh xl];simpl ww_to_Z;intros H.
    unfold Zlt in H;discriminate H.
    assert (H0 := spec_compare w_0 xh);rewrite spec_w_0 in H0.
-   simpl Z_of_N; destruct (w_compare w_0 xh).
+   destruct (w_compare w_0 xh).
    rewrite <- H0. simpl Zplus. rewrite <- H0 in H;simpl in H.
-   generalize (spec_w_head0 H);destruct (w_head0 xl) as [ |q].
-   intros H1;simpl Zpower in H1;rewrite Zmult_1_l in H1.
-   change (2 ^ Z_of_N (Npos w_digits)) with wB;split;zarith.
-   rewrite Zpower_2; apply Zmult_lt_compat_l;zarith.
-   unfold Z_of_N;intros.
-   change (Zpos(w_digits + q))with (Zpos w_digits + Zpos q);rewrite Zpower_exp.
-   fold wB;rewrite <- Zmult_assoc;split;zarith.
-   rewrite Zpower_2; apply Zmult_lt_compat_l;zarith.
-   intro H2;discriminate H2. intro H2;discriminate H2.
+   case (spec_to_Z w_zdigits); 
+     case (spec_to_Z (w_head0 xl)); intros HH1 HH2 HH3 HH4.
+   rewrite spec_w_add.
+   rewrite spec_zdigits; rewrite Zpower_exp; auto with zarith.
+   case (spec_w_head0 H); intros H1 H2.
+   rewrite Zpower_2; fold wB; rewrite <- Zmult_assoc; split.
+     apply Zmult_le_compat_l; auto with zarith.
+   apply Zmult_lt_compat_l; auto with zarith.
    assert (H1 := spec_w_head0 H0).
+   rewrite spec_w_0W.
    split.
    rewrite Zmult_plus_distr_r;rewrite Zmult_assoc.
-   apply Zle_trans with (2 ^ Z_of_N (w_head0 xh) * [|xh|] * wB).
-   rewrite Zmult_comm;zarith.
-   assert (0 <= 2 ^ Z_of_N (w_head0 xh) * [|xl|]);zarith.
+   apply Zle_trans with (2 ^ [|w_head0 xh|] * [|xh|] * wB).
+   rewrite Zmult_comm; zarith.
+   assert (0 <= 2 ^ [|w_head0 xh|] * [|xl|]);zarith.
    assert (H2:=spec_to_Z xl);apply Zmult_le_0_compat;zarith.
-   assert (0<= Z_of_N (w_head0 xh)).
-    case (w_head0 xh);intros;simpl;intro H2;discriminate H2.
-   generalize (Z_of_N (w_head0 xh)) H1 H2;clear H1 H2;intros p H1 H2.
+   case (spec_to_Z (w_head0 xh)); intros H2 _.
+   generalize ([|w_head0 xh|]) H1 H2;clear H1 H2;
+     intros p H1 H2.
    assert (Eq1 : 2^p < wB).
      rewrite <- (Zmult_1_r (2^p));apply Zle_lt_trans with (2^p*[|xh|]);zarith.
    assert (Eq2: p < Zpos w_digits).
@@ -150,59 +172,62 @@ Section GenLift.
     (wB_div w_digits w_to_Z spec_to_Z) 
     (wB_div_plus w_digits w_to_Z spec_to_Z) : w_rewrite.
   Ltac w_rewrite := autorewrite with w_rewrite;trivial.
- 
+
   Lemma spec_ww_add_mul_div_aux : forall xh xl yh yl p,
-     Zpos p < Zpos (xO w_digits) ->
-      [[match (p ?= w_digits)%positive Eq with
+   let zdigits := w_0W w_zdigits in
+    [[p]] <= Zpos (xO w_digits) ->
+      [[match ww_compare p zdigits with
         | Eq => w_WW xl yh
-        | Lt => w_WW (w_add_mul_div p xh xl) (w_add_mul_div p xl yh)
+        | Lt => w_WW (w_add_mul_div (low p) xh xl) 
+                     (w_add_mul_div (low p) xl yh)
         | Gt =>
-            let n := (p - w_digits)%positive in
+              let n := low (ww_sub p zdigits) in
             w_WW (w_add_mul_div n xl yh) (w_add_mul_div n yh yl)
         end]] =  
-      ([[WW xh xl]] * (2^Zpos p) +
-       [[WW yh yl]] / (2^(Zpos (xO w_digits) - Zpos p))) mod wwB.
+      ([[WW xh xl]] * (2^[[p]]) +
+       [[WW yh yl]] / (2^(Zpos (xO w_digits) - [[p]]))) mod wwB.
   Proof.
-   intros xh xl yh yl p;assert (HwwB := wwB_pos w_digits).
-   assert (0 < Zpos p). unfold Zlt;reflexivity.
+   intros xh xl yh yl p zdigits;assert (HwwB := wwB_pos w_digits).
+   case (spec_to_w_Z p); intros Hv1 Hv2.
    replace (Zpos (xO w_digits)) with (Zpos w_digits + Zpos w_digits).
    2 : rewrite Zpos_xO;ring.
-   replace (Zpos w_digits + Zpos w_digits - Zpos p) with 
-     (Zpos w_digits + (Zpos w_digits - Zpos p)). 2:ring.
+   replace (Zpos w_digits + Zpos w_digits - [[p]]) with 
+     (Zpos w_digits + (Zpos w_digits - [[p]])). 2:ring.
    intros Hp; assert (Hxh := spec_to_Z xh);assert (Hxl:=spec_to_Z xl);
    assert (Hx := spec_ww_to_Z w_digits w_to_Z spec_to_Z (WW xh xl));
    simpl in Hx;assert (Hyh := spec_to_Z yh);assert (Hyl:=spec_to_Z yl);
    assert (Hy:=spec_ww_to_Z w_digits w_to_Z spec_to_Z (WW yh yl));simpl in Hy.
-   case_eq  ((p ?= w_digits)%positive Eq);intros;w_rewrite;
-    match goal with 
-    | [H: (p ?= w_digits)%positive Eq = Eq |- _] =>
-      let H1:= fresh "H" in
-      (assert (H1 : Zpos p = Zpos w_digits);
-       [ rewrite Pcompare_Eq_eq with (1:= H);trivial
-       | rewrite H1;try rewrite Zminus_diag;try rewrite Zplus_0_r]);
-      fold wB
-    | [H: (p ?= w_digits)%positive Eq = Lt |- _] =>
-      change ((p ?= w_digits)%positive Eq = Lt) with 
-      (Zpos p < Zpos w_digits) in H;
-      repeat rewrite spec_w_add_mul_div;zarith
-    | [H: (p ?= w_digits)%positive Eq = Gt |- _] =>
-      change ((p ?= w_digits)%positive Eq=Gt)with(Zpos p > Zpos w_digits) in H;
-      let H1 := fresh "H" in
-      assert (H1 := Zpos_minus _ _ (Zgt_lt _ _ H));
-      replace (Zpos w_digits + (Zpos w_digits - Zpos p)) with
-       (Zpos w_digits - Zpos (p - w_digits));
-      [ repeat rewrite spec_w_add_mul_div;zarith
-      | zarith ] 
-    | _ => idtac
-    end;simpl ww_to_Z;w_rewrite;zarith.
+   generalize (spec_ww_compare p zdigits); case ww_compare; intros H1.
+   rewrite H1; unfold zdigits; rewrite spec_w_0W.
+   rewrite spec_zdigits; rewrite Zminus_diag; rewrite Zplus_0_r.
+   simpl ww_to_Z; w_rewrite;zarith.
+   fold wB.
    rewrite Zmult_plus_distr_l;rewrite <- Zmult_assoc;rewrite <- Zplus_assoc.
    rewrite <- Zpower_2.
    rewrite <- wwB_wBwB;apply Zmod_unique with [|xh|]. apply lt_0_wwB. 
    exact (spec_ww_to_Z w_digits w_to_Z spec_to_Z (WW xl yh)). ring.
+   simpl ww_to_Z; w_rewrite;zarith.
+   assert (HH0: [|low p|] = [[p]]).
+     rewrite spec_low.
+     apply Zmod_def_small.
+     case (spec_to_w_Z p); intros HH1 HH2; split; auto.
+     generalize H1; unfold zdigits; rewrite spec_w_0W;
+      rewrite spec_zdigits; intros tmp.
+     apply Zlt_le_trans with (1 := tmp).
+     unfold base.
+     apply Zpower2_le_lin; auto with zarith.
+   2: generalize H1; unfold zdigits; rewrite spec_w_0W;
+      rewrite spec_zdigits; auto with zarith.
+   generalize H1; unfold zdigits; rewrite spec_w_0W;
+      rewrite spec_zdigits; auto; clear H1; intros H1.
+   assert (HH: [|low p|] <= Zpos w_digits).
+     rewrite HH0; auto with zarith.
+   repeat rewrite spec_w_add_mul_div with (1 := HH).
+   rewrite HH0.
    rewrite Zmult_plus_distr_l.
-   pattern ([|xl|] * 2 ^ Zpos p) at 2;
+   pattern ([|xl|] * 2 ^ [[p]]) at 2;
    rewrite shift_unshift_mod with (n:= Zpos w_digits);fold wB;zarith.
-   replace ([|xh|] * wB * 2^Zpos p) with ([|xh|] * 2^Zpos p * wB). 2:ring. 
+   replace ([|xh|] * wB * 2^[[p]]) with ([|xh|] * 2^[[p]] * wB). 2:ring. 
    rewrite Zplus_assoc;rewrite <- Zmult_plus_distr_l. rewrite <- Zplus_assoc.
    unfold base at 5;rewrite <- Zmod_shift_r;zarith.
    unfold base;rewrite Zmod_shift_r with (b:= Zpos (ww_digits w_digits));
@@ -211,14 +236,40 @@ Section GenLift.
    unfold ww_digits;rewrite Zpos_xO;zarith. apply Z_mod_lt;zarith.
    split;zarith. apply Zdiv_lt_upper_bound;zarith.
    rewrite <- Zpower_exp;zarith.
-   ring_simplify (Zpos p + (Zpos w_digits - Zpos p));fold wB;zarith.
+   ring_simplify ([[p]] + (Zpos w_digits - [[p]]));fold wB;zarith.
+   assert (Hv: [[p]] > Zpos w_digits).
+     generalize H1; clear H1.
+     unfold zdigits; rewrite spec_w_0W; rewrite spec_zdigits; auto.
+   clear H1.
+   assert (HH0: [|low (ww_sub p zdigits)|] = [[p]] - Zpos w_digits).
+     rewrite spec_low.
+     rewrite spec_ww_sub.
+     unfold zdigits; rewrite spec_w_0W; rewrite spec_zdigits.
+     rewrite <- Zmod_div_mod; auto with zarith.
+     rewrite Zmod_def_small; auto with zarith.
+     split; auto with zarith.
+     apply Zle_lt_trans with (Zpos w_digits); auto with zarith.
+     unfold base; apply Zpower2_lt_lin; auto with zarith.
+     exists wB; unfold base.
+     unfold ww_digits; rewrite (Zpos_xO w_digits).
+     rewrite <- Zpower_exp; auto with zarith.
+     apply f_equal with (f := fun x => 2 ^ x); auto with zarith.
+   assert (HH: [|low (ww_sub p zdigits)|] <= Zpos w_digits).
+     rewrite HH0; auto with zarith.
+   replace (Zpos w_digits + (Zpos w_digits - [[p]])) with
+       (Zpos w_digits - ([[p]] - Zpos w_digits)); zarith.
+   lazy zeta; simpl ww_to_Z; w_rewrite;zarith.
+   repeat rewrite spec_w_add_mul_div;zarith.
+   rewrite HH0.
    pattern wB at 5;replace wB with 
-    (2^(Zpos (p - w_digits) + (Zpos w_digits - Zpos (p - w_digits)))).
+    (2^(([[p]] - Zpos w_digits) 
+         + (Zpos w_digits - ([[p]] - Zpos w_digits)))).
    rewrite Zpower_exp;zarith. rewrite Zmult_assoc.
    rewrite Z_div_plus_l;zarith.
-   rewrite shift_unshift_mod with (a:= [|yh|]) (p:= Zpos (p - w_digits))
+   rewrite shift_unshift_mod with (a:= [|yh|]) (p:= [[p]] - Zpos w_digits)
     (n := Zpos w_digits);zarith. fold wB.
-   replace (Zpos p) with (Zpos (p - w_digits) + Zpos w_digits);zarith.
+   set (u := [[p]] - Zpos w_digits).
+   replace [[p]] with (u + Zpos w_digits);zarith.
    rewrite Zpower_exp;zarith. rewrite Zmult_assoc. fold wB.
    repeat rewrite Zplus_assoc. rewrite <- Zmult_plus_distr_l.
    repeat rewrite <- Zplus_assoc.
@@ -228,30 +279,36 @@ Section GenLift.
    (b:= Zpos w_digits);fold wB;fold wwB;zarith.
    rewrite wwB_wBwB; rewrite Zpower_2; rewrite  Zmult_mod_distr_r;zarith.
    rewrite Zmult_plus_distr_l.
-   replace ([|xh|] * wB * 2 ^ Zpos (p - w_digits)) with 
-     ([|xh|]*2^Zpos(p - w_digits)*wB). 2:ring.
+   replace ([|xh|] * wB * 2 ^ u) with 
+     ([|xh|]*2^u*wB). 2:ring.
    repeat rewrite <- Zplus_assoc. 
-   rewrite (Zplus_comm ([|xh|] * 2 ^ Zpos (p - w_digits) * wB)).
+   rewrite (Zplus_comm ([|xh|] * 2 ^ u * wB)).
    rewrite Z_mod_plus;zarith. rewrite Zmod_mult_0;zarith.
    unfold base;rewrite <- Zmod_shift_r;zarith. fold base;apply Z_mod_lt;zarith.
-   split;zarith. apply Zdiv_lt_upper_bound;zarith.
-   rewrite <- Zpower_exp;zarith. 
-   ring_simplify (Zpos (p - w_digits) + (Zpos w_digits - Zpos (p - w_digits))); fold 
+   unfold u; split;zarith. 
+   split;zarith. unfold u; apply Zdiv_lt_upper_bound;zarith.
+   rewrite <- Zpower_exp;zarith.
+   fold u. 
+   ring_simplify (u + (Zpos w_digits - u)); fold 
    wB;zarith. unfold ww_digits;rewrite Zpos_xO;zarith.
    unfold base;rewrite <- Zmod_shift_r;zarith. fold base;apply Z_mod_lt;zarith.
-   split;zarith. apply Zdiv_lt_upper_bound;zarith.
-   rewrite <- Zpower_exp;zarith. 
-   ring_simplify (Zpos (p - w_digits) + (Zpos w_digits - Zpos (p - w_digits))); fold 
-   wB;zarith. 
-   ring_simplify (Zpos (p - w_digits) + (Zpos w_digits - Zpos (p - w_digits))); fold 
-   wB;trivial.
+   unfold u; split;zarith.
+   unfold u; split;zarith.
+   apply Zdiv_lt_upper_bound;zarith.
+   rewrite <- Zpower_exp;zarith.
+   fold u. 
+   ring_simplify (u + (Zpos w_digits - u)); fold wB; auto with zarith.
+   unfold u;zarith.
+   unfold u;zarith.
+   set (u := [[p]] - Zpos w_digits).
+   ring_simplify (u + (Zpos w_digits - u)); fold wB; auto with zarith.
   Qed.
 
   Lemma spec_ww_add_mul_div : forall x y p,
-       Zpos p < Zpos (xO w_digits) ->
+       [[p]] <= Zpos (xO w_digits) ->
        [[ ww_add_mul_div p x y ]] =
-         ([[x]] * (2^Zpos p) +
-          [[y]] / (2^(Zpos (xO w_digits) - Zpos p))) mod wwB.
+         ([[x]] * (2^[[p]]) +
+          [[y]] / (2^(Zpos (xO w_digits) - [[p]]))) mod wwB.
   Proof.
    intros x y p H.
    destruct x as [ |xh xl];
@@ -261,15 +318,40 @@ Section GenLift.
     [generalize (H1 w_0 w_0 p H) | generalize (H1 yh yl p H)];
     clear H1;w_rewrite);simpl ww_add_mul_div.
    replace [[WW w_0 w_0]] with 0;[w_rewrite|simpl;w_rewrite;trivial].
-   intros Heq;rewrite <- Heq;clear Heq.
-   case_eq ((p ?= w_digits)%positive Eq);w_rewrite;intros;trivial.
+   intros Heq;rewrite <- Heq;clear Heq; auto.
+   generalize (spec_ww_compare p (w_0W w_zdigits)); 
+     case ww_compare; intros H1; w_rewrite.
    rewrite (spec_w_add_mul_div w_0 w_0);w_rewrite;zarith.
+   generalize H1; w_rewrite; rewrite spec_zdigits; clear H1; intros H1.
+   assert (HH0: [|low p|] = [[p]]).
+     rewrite spec_low.
+     apply Zmod_def_small.
+     case (spec_to_w_Z p); intros HH1 HH2; split; auto.
+     apply Zlt_le_trans with (1 := H1).
+     unfold base; apply Zpower2_le_lin; auto with zarith.
+   rewrite HH0; auto with zarith.
    replace [[WW w_0 w_0]] with 0;[w_rewrite|simpl;w_rewrite;trivial].
    intros Heq;rewrite <- Heq;clear Heq.
-   case_eq ((p ?= w_digits)%positive Eq);w_rewrite;intros;trivial.
+   generalize (spec_ww_compare p (w_0W w_zdigits)); 
+     case ww_compare; intros H1; w_rewrite.
    rewrite (spec_w_add_mul_div w_0 w_0);w_rewrite;zarith.
-   change ((p ?= w_digits)%positive Eq = Gt)with(Zpos p > Zpos w_digits) in H0.
-   rewrite Zpos_minus;zarith. rewrite Zpos_xO in H;zarith.
+   rewrite Zpos_xO in H;zarith.
+   assert (HH: [|low (ww_sub p (w_0W w_zdigits)) |] = [[p]] - Zpos w_digits).
+     generalize H1; clear H1.
+     rewrite spec_low.
+     rewrite spec_ww_sub; w_rewrite; intros H1.
+     rewrite <- Zmod_div_mod; auto with zarith.
+     rewrite Zmod_def_small; auto with zarith.
+     split; auto with zarith.
+     apply Zle_lt_trans with (Zpos w_digits); auto with zarith.
+     unfold base; apply Zpower2_lt_lin; auto with zarith.
+     unfold base; auto with zarith.
+     unfold base; auto with zarith.
+     exists wB; unfold base.
+     unfold ww_digits; rewrite (Zpos_xO w_digits).
+     rewrite <- Zpower_exp; auto with zarith.
+     apply f_equal with (f := fun x => 2 ^ x); auto with zarith.
+  case (spec_to_Z xh); auto with zarith.
   Qed.
 
  End GenProof.
